theories/FileSystem.v
@@ -1,11 +1,39 @@
-From Coq Require Import Int63 String.
-From FreeSpec Require Import Core Files.
+From Coq Require Import Int63.
+From Prelude Require Import All Bytes Text.
+From FreeSpec Require Import Core.
+From Praecia Require Import Init.
 
 Generalizable All Variables.
 
 (** * Definition  *)
 
+Axiom file_descriptor : Type.
 Axiom fd_eq_dec : forall (fd1 fd2 : file_descriptor), { fd1 = fd2 } + { ~ (fd1 = fd2) }.
+
+
+Inductive FILESYSTEM : interface :=
+| Open (path : bytes) : FILESYSTEM file_descriptor
+| FileExists (file : bytes) : FILESYSTEM bool
+| Read (file : file_descriptor) : FILESYSTEM bytes
+| Close (file : file_descriptor) : FILESYSTEM unit.
+
+Register FILESYSTEM as praecia.filesystem.type.
+Register Open as praecia.filesystem.Open.
+Register FileExists as praecia.filesystem.FileExists.
+Register Read as praecia.filesystem.Read.
+Register Close as praecia.filesystem.Close.
+
+Definition open `{Provide ix FILESYSTEM} (path : bytes) : impure ix file_descriptor :=
+  request (Open path).
+
+Definition close `{Provide ix FILESYSTEM} (fd : file_descriptor) : impure ix unit :=
+  request (Close fd).
+
+Definition file_exists `{Provide ix FILESYSTEM} (path : bytes) : impure ix bool :=
+  request (FileExists path).
+
+Definition read `{Provide ix FILESYSTEM} (fd : file_descriptor) : impure ix bytes :=
+  request (Read fd).
 
 (** * Contracts *)
 
@@ -32,7 +60,7 @@ Proof.
   now rewrite m in a.
 Qed.
 
-Hint Resolve member_not_absent.
+Hint Resolve member_not_absent : praecia.
 
 Lemma absent_not_member (ω : fd_set) (fd : file_descriptor)
   : absent ω fd -> ~ member ω fd.
@@ -43,7 +71,7 @@ Proof.
   now rewrite m in a.
 Qed.
 
-Hint Resolve absent_not_member.
+Hint Resolve absent_not_member : praecia.
 
 Lemma member_add_fd (ω : fd_set) (fd : file_descriptor) : member (add_fd ω fd) fd.
 
@@ -52,49 +80,47 @@ Proof.
   destruct fd_eq_dec; auto.
 Qed.
 
-Hint Resolve member_add_fd.
+Hint Resolve member_add_fd : praecia.
 
-Definition fd_set_update (ω : fd_set) (a : Type) (e : FILES a) (x : a) : fd_set :=
+Definition fd_set_update (ω : fd_set) (a : Type) (e : FILESYSTEM a) (x : a) : fd_set :=
   match e, x with
-  | Open _, inr fd =>
+  | Open _, fd =>
     add_fd ω fd
   | Close fd, _ =>
     del_fd ω fd
-  | Read _ _, _ =>
+  | Read _, _ =>
     ω
-  | FSize _, _ =>
-    ω
-  | Open _, _ =>
+  | FileExists _, _ =>
     ω
   end.
 
-Inductive fd_set_caller_obligation (ω : fd_set) : forall (a : Type), FILES a -> Prop :=
-| fd_set_open_caller (p : string)
-  : fd_set_caller_obligation ω _ (Open p)
-| fd_set_read_caller (fd : file_descriptor) (n : int) (is_member : member ω fd)
-  : fd_set_caller_obligation ω _ (Read fd n)
+
+Inductive fd_set_caller_obligation (ω : fd_set) : forall (a : Type), FILESYSTEM a -> Prop :=
+| fd_set_open_caller (p : bytes)
+  : fd_set_caller_obligation ω file_descriptor (Open p)
+| fd_set_read_caller (fd : file_descriptor) (is_member : member ω fd)
+  : fd_set_caller_obligation ω bytes (Read fd)
 | fd_set_close_caller (fd : file_descriptor) (is_member : member ω fd)
   : fd_set_caller_obligation ω unit (Close fd)
-| fd_set_is_file_caller (fd : file_descriptor)
-  : fd_set_caller_obligation ω _ (FSize fd).
+| fd_set_is_file_caller (p : bytes)
+  : fd_set_caller_obligation ω bool (FileExists p).
 
-Hint Constructors fd_set_caller_obligation.
+Hint Constructors fd_set_caller_obligation : praecia.
 
-Inductive fd_set_callee_obligation (ω : fd_set) : forall (a : Type), FILES a -> a -> Prop :=
-| fd_set_open_callee_left (p : string) (fd : file_descriptor) (is_absent : absent ω fd)
-  : fd_set_callee_obligation ω _ (Open p) (inr fd)
-| fd_set_open_callee_right (p : string) (e : files_err)
-  : fd_set_callee_obligation ω _ (Open p) (inl e)
-| fd_set_read_callee (fd : file_descriptor) (n : int) (res : files_err + (int * string))
-  : fd_set_callee_obligation ω _ (Read fd n) res
+
+Inductive fd_set_callee_obligation (ω : fd_set) : forall (a : Type), FILESYSTEM a -> a -> Prop :=
+| fd_set_open_callee (p : bytes) (fd : file_descriptor) (is_absent : absent ω fd)
+  : fd_set_callee_obligation ω file_descriptor (Open p) fd
+| fd_set_read_callee (fd : file_descriptor) (s : bytes)
+  : fd_set_callee_obligation ω bytes (Read fd) s
 | fd_set_close_callee (fd : file_descriptor) (t : unit)
   : fd_set_callee_obligation ω unit (Close fd) t
-| fd_set_fsize_callee (fd : file_descriptor) (res : files_err + int)
-  : fd_set_callee_obligation ω _ (FSize fd) res.
+| fd_set_is_file_callee (p : bytes) (b : bool)
+  : fd_set_callee_obligation ω bool (FileExists p) b.
 
-Hint Constructors fd_set_callee_obligation.
+Hint Constructors fd_set_callee_obligation : praecia.
 
-Definition fd_set_contract : contract FILES fd_set :=
+Definition fd_set_contract : contract FILESYSTEM fd_set :=
   {| witness_update := fd_set_update
    ; caller_obligation := fd_set_caller_obligation
    ; callee_obligation := fd_set_callee_obligation
