theories/Server.v
@@ -1,58 +1,71 @@
-From FreeSpec Require Import Core Core.Notations.
-From Praecia Require Import FileSystem TCP URI HTTP Parser.
-From Prelude Require Import Tactics.
-
-Import ListNotations.
-#[local] Open Scope string_scope.
-#[local] Open Scope prelude_scope.
-
-#[local] Opaque http_request.
+From Coq Require Import FunctionalExtensionality.
+From FreeSpec Require Import Core Console.
+From Praecia Require Import FileSystem TCP URI HTTP.
+From Prelude Require Import All Tactics Bytes Text.
 
 Generalizable All Variables.
 
 Definition sandbox (base : list directory_id) (req : uri) : uri :=
   make_uri (List.app base (canonicalize (dirname req))) (filename req).
 
-Definition read_content `{Provide ix FILESYSTEM} (path : string)
-  : impure ix string :=
-  open path >>= fun fd => read fd <* close fd.
+Definition read_content `{Provide2 ix FILESYSTEM CONSOLE}
+    (path : bytes)
+  : impure ix bytes :=
+  do echo ("  reading <" ++ path ++ ">... ");
+     let* fd <- open path in
+     let* c <- read fd in
+     close fd;
+     echo ("done.\n");
+     pure c
+  end.
 
 (* TODO: add a notation in coq-prelude var (x : T) <- p in q *)
-Definition request_handler `{Provide ix FILESYSTEM}
+Definition request_handler `{Provide2 ix FILESYSTEM CONSOLE}
     (base : list directory_id) (req : request)
   : impure ix response :=
   match req with
   | Get uri =>
     do let path := uri_to_path (sandbox base uri) in
-       var isf <- file_exists path in
+       let* isf <- file_exists path in
        if (isf : bool)
        then make_response success_OK <$> read_content path
-       else pure (make_response client_error_NotFound "Resource not found.")
+       else do echo ("  resource <" ++ path ++"> not found\n");
+               pure (make_response client_error_NotFound "Resource not found.")
+            end
     end
   end.
 
-Definition tcp_handler `{Provide ix FILESYSTEM}
-    (base : list directory_id) (req : string)
-  : impure ix string :=
-  response_to_string <$> match parse http_request req with
-                         | inl _ => pure (make_response client_error_BadRequest "")
-                         | inr req => request_handler base req
-                         end.
+Definition tcp_handler `{Provide2 ix FILESYSTEM CONSOLE}
+    (base : list directory_id) (req : bytes)
+  : impure ix bytes :=
+  do echo "new request received\n";
+     echo ("  request size is " ++ Int.bytes_of_int (Bytes.length req) ++ "\n");
+     response_to_string <$> match http_request req with
+                            | inl _ => pure (make_response client_error_BadRequest "Bad request")
+                            | inr req => request_handler base (fst req)
+                            end
+  end.
 
-Definition http_server `{Provide ix FILESYSTEM, Provide ix TCP}
+Definition http_server `{Provide3 ix FILESYSTEM TCP CONSOLE}
   : impure ix unit :=
-  tcp_server (tcp_handler [Dirname "tmp"]).
+  do echo "hello, world!\n";
+     tcp_server (tcp_handler [Dirname "tmp"])
+  end.
 
-Lemma fd_set_respectful_read_content `{Provide ix FILESYSTEM} (ω : fd_set) (path : string)
+#[local] Opaque http_request.
+
+Tactic Notation "prove" "impure" "with" ident(db) := prove_impure; eauto with db.
+
+Lemma fd_set_respectful_read_content `{StrictProvide2 ix FILESYSTEM CONSOLE} (ω : fd_set) (path : bytes)
   : respectful_impure fd_set_contract ω (read_content path).
 
 Proof.
-  now prove_impure.
+  prove impure with praecia.
 Qed.
 
-Hint Resolve fd_set_respectful_read_content.
+Hint Resolve fd_set_respectful_read_content : praecia.
 
-Lemma fd_set_preserving_read_content `{Provide ix FILESYSTEM} (path : string)
+Lemma fd_set_preserving_read_content `{StrictProvide2 ix FILESYSTEM CONSOLE} (path : bytes)
   : fd_set_preserving (read_content path).
 
 Proof.
@@ -61,22 +74,22 @@ Proof.
   intros fd'.
   unfold add_fd, del_fd.
   destruct fd_eq_dec; subst.
-  + now inversion o_callee; ssubst.
+  + now inversion o_callee0; ssubst.
   + reflexivity.
 Qed.
 
 #[local] Opaque read_content.
 
-Lemma fd_set_respectful_file_exists `{Provide ix FILESYSTEM} (ω : fd_set) (path : string)
+Lemma fd_set_respectful_file_exists `{Provide ix FILESYSTEM} (ω : fd_set) (path : bytes)
   : respectful_impure fd_set_contract ω (file_exists path).
 
 Proof.
-  now prove_impure.
+  prove impure with praecia.
 Qed.
 
-Hint Resolve fd_set_respectful_file_exists.
+Hint Resolve fd_set_respectful_file_exists : praecia.
 
-Lemma fd_set_preserving_file_exists `{Provide ix FILESYSTEM} (path : string)
+Lemma fd_set_preserving_file_exists `{Provide ix FILESYSTEM} (path : bytes)
   : fd_set_preserving (file_exists path).
 
 Proof.
@@ -86,8 +99,8 @@ Qed.
 
 #[local] Opaque file_exists.
 
-Lemma fd_set_respectful_tcp_handler `{Provide ix FILESYSTEM}
-    (base : list directory_id) (req : string) (ω : fd_set)
+Lemma fd_set_respectful_tcp_handler `{StrictProvide2 ix FILESYSTEM CONSOLE}
+    (base : list directory_id) (req : bytes) (ω : fd_set)
   : respectful_impure fd_set_contract ω (tcp_handler base req).
 
 Proof.
@@ -96,35 +109,32 @@ Proof.
   + prove_impure.
   + prove_impure.
     destruct (fst p).
-    now prove_impure.
+    prove impure with praecia.
 Qed.
 
-Hint Resolve fd_set_respectful_tcp_handler.
+Hint Resolve fd_set_respectful_tcp_handler : praecia.
 
-Lemma fd_set_preserving_tcp_handler `{Provide ix FILESYSTEM}
-    (base : list directory_id) (req : string)
+Lemma fd_set_preserving_tcp_handler `{StrictProvide2 ix FILESYSTEM CONSOLE}
+    (base : list directory_id) (req : bytes)
   : fd_set_preserving (tcp_handler base req).
 
 Proof.
   intros ω ω' x run fd.
   unroll_respectful_run run.
   destruct (http_request req).
-  + now unroll_respectful_run run0.
+  + now unroll_respectful_run run.
   + destruct p as [[res_id] req'].
-    unroll_respectful_run run0.
-    ++ apply fd_set_preserving_file_exists in run.
-       apply fd_set_preserving_read_content in run0.
-
+    unroll_respectful_run run.
+    ++ apply fd_set_preserving_file_exists in run0.
+       apply fd_set_preserving_read_content in run.
        now transitivity (ω'' fd).
-    ++ now apply fd_set_preserving_file_exists in run.
+    ++ now apply fd_set_preserving_file_exists in run0.
 Qed.
 
-Hint Resolve fd_set_preserving_tcp_handler.
+Hint Resolve fd_set_preserving_tcp_handler : praecia.
 
 #[local] Opaque tcp_handler.
 #[local] Opaque response_to_string.
-
-From Coq Require Import FunctionalExtensionality.
 
 Lemma fd_set_preserving_repeatM {a} `{Provide ix FILESYSTEM}
     (p : impure ix a)
@@ -140,13 +150,12 @@ Proof.
     apply IHn.
     assert (equ : ω = ω''). {
       apply functional_extensionality.
-      intros fd'.
-      eapply (fd_preserving ω); eauto.
+      eauto with praecia.
     }
     now rewrite equ.
 Qed.
 
-Hint Resolve fd_set_preserving_repeatM.
+Hint Resolve fd_set_preserving_repeatM : praecia.
 
 Lemma repeatM_preserving_respectful {a} `{Provide ix FILESYSTEM}
     (p : impure ix a) (ω : fd_set)
@@ -175,12 +184,12 @@ Qed.
 Lemma fd_set_preserving_tcp_server_repeat_routine
    `{Provide ix TCP, MayProvide ix FILESYSTEM, Distinguish ix TCP FILESYSTEM}
     (server : socket_descriptor)
-    (handler : string -> impure ix string)
-    (preserve : forall (req : string), fd_set_preserving (handler req))
-  : fd_set_preserving (do var client <- accept_connection server in
+    (handler : bytes -> impure ix bytes)
+    (preserve : forall (req : bytes), fd_set_preserving (handler req))
+  : fd_set_preserving (do let* client <- accept_connection server in
 
-                          var req <- read_socket client in
-                          var res <- handler req in
+                          let* req <- read_socket client in
+                          let* res <- handler req in
                           write_socket client res;
 
                           close_socket client
@@ -192,26 +201,30 @@ Proof.
   now apply preserve in run.
 Qed.
 
-Hint Resolve fd_set_preserving_tcp_server_repeat_routine.
+Hint Resolve fd_set_preserving_tcp_server_repeat_routine : praecia.
 
-Lemma fd_set_respectful_http_server `{StrictProvide2 ix FILESYSTEM TCP} (ω : fd_set)
+Lemma fd_set_respectful_http_server `{StrictProvide3 ix FILESYSTEM TCP CONSOLE}
+    (ω : fd_set)
   : respectful_impure fd_set_contract ω http_server.
 
 Proof.
   prove_impure.
   apply repeatM_preserving_respectful.
   + prove_impure.
-    destruct (http_request x2); now prove_impure.
+    destruct (http_request x3); prove impure with praecia;
+       apply fd_set_respectful_tcp_handler. (* TODO: Why do we need this when it has been added as a hint? *)
   + intros ω' ω'' [] run fd.
-    apply fd_set_preserving_tcp_server_repeat_routine in run; auto.
+    apply fd_set_preserving_tcp_server_repeat_routine in run; auto with praecia.
+    apply fd_set_preserving_tcp_handler. (* TODO: Same here? *)
 Qed.
 
-Lemma fd_set_preserving_http_server `{StrictProvide2 ix FILESYSTEM TCP}
+Lemma fd_set_preserving_http_server `{StrictProvide3 ix FILESYSTEM TCP CONSOLE}
   : fd_set_preserving http_server.
 
 Proof.
   intros ω ω' x run fd.
   unroll_respectful_run run.
-  apply fd_set_preserving_repeatM in run; auto.
-  now apply fd_set_preserving_tcp_server_repeat_routine.
+  apply fd_set_preserving_repeatM in run; auto with praecia.
+  apply fd_set_preserving_tcp_server_repeat_routine.
+  apply fd_set_preserving_tcp_handler.
 Qed.
