theories/TCP.v
@@ -1,4 +1,4 @@
-From Coq Require Export String.
+From Prelude Require Import All Bytes Text.
 From FreeSpec Require Export Core Exec.
 
 Generalizable All Variables.
@@ -6,11 +6,11 @@ Generalizable All Variables.
 Axiom socket_descriptor : Type.
 
 Inductive TCP : interface :=
-| NewTCPSocket (addr : string) : TCP socket_descriptor
+| NewTCPSocket (addr : bytes) : TCP socket_descriptor
 | ListenIncomingConnection (socket : socket_descriptor) : TCP unit
 | AcceptConnection (socket : socket_descriptor) : TCP socket_descriptor
-| ReadSocket (socket : socket_descriptor) : TCP string
-| WriteSocket (socket : socket_descriptor) (msg : string) : TCP unit
+| ReadSocket (socket : socket_descriptor) : TCP bytes
+| WriteSocket (socket : socket_descriptor) (msg : bytes) : TCP unit
 | CloseTCPSocket (socket : socket_descriptor) : TCP unit.
 
 Register TCP as praecia.tcp.type.
@@ -21,7 +21,7 @@ Register ReadSocket as praecia.tcp.ReadSocket.
 Register WriteSocket as praecia.tcp.WriteSocket.
 Register CloseTCPSocket as praecia.tcp.CloseTCPSocket.
 
-Definition new_tcp_socket `{Provide ix TCP} (addr : string) : impure ix socket_descriptor :=
+Definition new_tcp_socket `{Provide ix TCP} (addr : bytes) : impure ix socket_descriptor :=
   request (NewTCPSocket addr).
 
 Definition listen_incoming_connection `{Provide ix TCP} (socket : socket_descriptor) : impure ix unit :=
@@ -30,33 +30,31 @@ Definition listen_incoming_connection `{Provide ix TCP} (socket : socket_descrip
 Definition accept_connection `{Provide ix TCP} (socket : socket_descriptor) : impure ix socket_descriptor :=
   request (AcceptConnection socket).
 
-Definition read_socket `{Provide ix TCP} (socket : socket_descriptor) : impure ix string :=
+Definition read_socket `{Provide ix TCP} (socket : socket_descriptor) : impure ix bytes :=
   request (ReadSocket socket).
 
-Definition write_socket `{Provide ix TCP} (socket : socket_descriptor) (msg : string) : impure ix unit :=
+Definition write_socket `{Provide ix TCP} (socket : socket_descriptor) (msg : bytes) : impure ix unit :=
   request (WriteSocket socket msg).
 
 Definition close_socket `{Provide ix TCP} (socket : socket_descriptor) : impure ix unit :=
   request (CloseTCPSocket socket).
 
-Declare ML Module "praecia_plugin".
-
 Fixpoint repeatM `{Monad m} {a} (n : nat) (p : m a) : m unit :=
   match n with
   | O => pure tt
-  | S n => p >>= fun _ => repeatM n p
+  | S n => do p >>= fun _ => repeatM n p end
   end.
 
-Definition tcp_server `{Provide ix TCP} (handler : string -> impure ix string)
+Definition tcp_server `{Provide ix TCP} (handler : bytes -> impure ix bytes)
   : impure ix unit :=
-  do var server <- new_tcp_socket "127.0.0.1:8088" in
+  do let* server <- new_tcp_socket (bytes_of_text "127.0.0.1:8088") in
      listen_incoming_connection server;
 
      repeatM 100 do
-       var client <- accept_connection server in
+       let* client <- accept_connection server in
 
-       var req <- read_socket client in
-       var res <- handler req in
+       let* req <- read_socket client in
+       let* res <- handler req in
        write_socket client res;
 
        close_socket client
