theories/Exec.v
@@ -1,0 +1,4 @@
+From FreeSpec Require Import Core Exec.
+From Praecia Require Import TCP FileSystem.
+
+Declare ML Module "praecia_plugin".
